Законы.

1.

$$ A \wedge  B = B \wedge  A $$

3

$$ A\bigwedge_{}^{}(B\bigwedge_{}^{}C)=(A\bigwedge_{}^{}B)\bigwedge_{}^{}C $$

4

$$ (A \bigvee_{}^{} B) \bigvee C = A \bigvee(B \bigvee C) $$

5

$$ (A\bigwedge_{}^{}B)\bigvee_{}^{}C=(A\bigvee_{}^{}C)\bigwedge_{}^{}(B\bigvee_{}^{}C) $$

6

$$ (A \bigvee B) \bigwedge C=(A \bigwedge C) \bigvee (B \bigwedge C) $$

13

$$ A \wedge (A \bigvee_{}^{} B) = A $$

14 

$$ A \wedge(A \vee B) = A $$

15


16 

$$ \overline{(a \wedge b)} = \overline{a} \vee \overline{b} $$

17 

$$ \(\bar {\bar A}=A\) $$

18


19 

$$ A\leftrightarrow B=(\bar{A} {\vee } B)\wedge (\bar{B} \vee A) $$

20

$$ A \oplus B = (\bar{A} \wedge  B) \vee (A \wedge  \bar{B)} $$
